\section{Old exam 2021-01-11}

\begin{enumerate}[label=\arabic*., leftmargin=*]
  \setcounter{enumi}{1}
  \item
  \begin{enumerate}[label=\alph*),leftmargin=*]
    \item A useful model could  be $\underbrace{X_ij}_{4\times 1} = \mu+\underbrace{\alpha_i}_{\text{brand}}+\varepsilon_{ij}$, here we test if the mean is the same across all $\alpha_i = 0\quad\forall i$
      \par\bigskip
    \item Mathematically, the testing proble can be expressed as the following:
      \begin{equation*}
        \begin{gathered}
          H_0:\alpha_i = 0\quad\forall i = 1,2,3,4
        \end{gathered}
      \end{equation*}
      \par\bigskip
      \noindent Identification restriction is given by $\Sigma\alpha_i = 0$
      \par\bigskip
    \item
      \begin{equation*}
        \begin{gathered}
          \sum_{i=1}^{4}\sum_{j}(X_{ij}-\overline{X})(X_{ij}-\overline{X})^T =B+W
        \end{gathered}
      \end{equation*}
      \par\bigskip
      \noindent Here the $B$ is the \textit{between } sum of squares (compares observations between groups)\par
      \noindent Here the $W$ is the \textit{within} sum of squares (compares observations between each group)
      \par\bigskip
    \item $H_=:\mu=\mu_0\qquad X_1,\cdots,X_n\sim N(\mu,\Sigma)$. Testing normal mean
  \end{enumerate}
  \par\bigskip
\item If $m\neq n$, then we can exclude the "paired data test" directly since they need to have the same dimensions 
  \par\bigskip
  \begin{enumerate}[label=\alph*),leftmargin=*]
    \item We are therefore testing $\mu_X=\mu_Y$ 
      \par\bigskip
    \item Only $S_{\text{pooled}}$ is for $2$-sample test (which is what we have for this case)\par
      \noindent What we do is assume $\Sigma_1 = \Sigma_2$ and estimate by Chapter 6 p.10:
      \begin{equation*}
        \begin{gathered}
          S_{\text{pooled}} = \dfrac{\sum_{j=1}^{n_1}(X_{1j}-\overline{X}_1)(X_{1j}-\overline{X}_1)^T+\sum_{j=1}^{n_2}(X_{2j}-\overline{X}_2)(X_{2j}-\overline{X}_2)^T}{n_1+n_2-2} = \dfrac{(n_1-1)S_1}{n_1+n_2-2}+ \dfrac{(n_2-1)S_2}{(n_1+n_2-2)}
        \end{gathered}
      \end{equation*}
      \par\bigskip
      \noindent Before we proceed with showing which distribution, it will be easier if we first do c) and then use the results here
      \par\bigskip
    \item 
      \begin{equation*}
        \begin{gathered}
          S_1 = \dfrac{1}{n-1}\sum(X_{ij}-\overline{X})(X_{ij}-\overline{X})^T\qquad\text{for unbiased}\\
          S_1 = \dfrac{1}{n}\sum(X_{ij}-\overline{X})(X_{ij}-\overline{X})^T\qquad\text{for MLE}\\
          \Rightarrow \sum_{j=1}^{n}(X_j-\overline{X})(X_j-\overline{X})^T\sim W_p(\Sigma,n-1)\\
          \Rightarrow S_1\text{ is Wishart }\Lrarr (n_1-1)S_1\text{ is Wishart}\\
          \Rightarrow S_{\text{pool}}\sim W_p(\Sigma,n_1-1)+W_p(\Sigma,n_2-1)\Rightarrow (n_1+n_2-2)S_{\text{pool}} = W_p(\Sigma,n_1+n_2-2)
        \end{gathered}
      \end{equation*}
      \par\bigskip
      \noindent Due to the independance, Wishart + Wishart is still Wishart.\par
      \noindent If we test the mean of the first sample, can we get Hotellings $T^2$?
      \begin{equation*}
        \begin{gathered}
          \overline{X}\sim N(\mu,\Sigma) \Rightarrow n(\overline{X}-\mu_X)\sim N(0,\Sigma)
        \end{gathered}
      \end{equation*}
      \par\bigskip
    \item $\Sigma$ is common for both samples. We shall use some results from $S_{\text{pool}}$:
      \begin{equation*}
        \begin{gathered}
          X_1,\cdots,X_{n_1}\sim N\left(\mu_X,\begin{bmatrix}\Sigma_{11}&\Sigma_{12}\\\Sigma_{21}&\Sigma_{22}\end{bmatrix}\right)\\
          Y_1,\cdots,Y_{n_2}\sim N\left(\mu_Y,\begin{bmatrix}\Sigma_{11}&\Sigma_{12}\\\Sigma_{21}&\Sigma_{22}\end{bmatrix}\right)
        \end{gathered}
      \end{equation*}
      \par\bigskip
      \noindent If we only care about $\Sigma_{11}$ then for every observation we take out the first 2 since:
      \begin{equation*}
        \begin{gathered}
          \forall X_i\quad \begin{bmatrix}X_{i1}\\X_{i2}\\X_{i3}\\X_{i4}\end{bmatrix}\rightarrow \begin{bmatrix}X_{i1}\\X_{i2}\end{bmatrix}\\
          \forall Y_i\quad \begin{bmatrix}Y_{i1}\\Y_{i2}\\Y_{i3}\\Y_{i4}\end{bmatrix}\rightarrow \begin{bmatrix}Y_{i1}\\Y_{i2}\end{bmatrix}
        \end{gathered}
      \end{equation*}
      \par\bigskip
      $\Rightarrow$ the estimator has distribution $W_2(\Sigma_{11},n_1+n_2-2)$ 
      \par\bigskip
    \item In order to use $ny^TM^{-1}y\sim T^2(\Sigma,n)$, we need $\overline{x}\sim N(0,\Sigma)$ and $M\sim W(\Sigma,n)$ (where they share $\Sigma$):
      \begin{equation*}
        \begin{gathered}
          \overline{x}\sim N(\mu,\Sigma_{11}/n)\Rightarrow \sqrt{n}(\overline{x}-\mu_1)\sim N(0,\Sigma_{11}) = y\\
          (n_1+n_2-2)S_{\text{pool}} = M
        \end{gathered}
      \end{equation*}
      \par\bigskip
      \noindent For two-sample testing:
      \begin{equation*}
        \begin{gathered}
          (\overline{x}-\overline{y})\sim N\left([\mu_{X_1}-\mu_{Y_1}],\left(\dfrac{1}{n_1}+\dfrac{1}{n_2}\right)\Sigma_{11}\right)\\
          \Rightarrow \dfrac{1}{\sqrt{\dfrac{1}{n_1}+\dfrac{1}{n_2}}}\left[\overline{x}-\overline{y}-(\mu_{X_1}-\mu_{Y_1})\right]\sim N(0,\Sigma_{11})
        \end{gathered}
      \end{equation*}
  \end{enumerate}
\end{enumerate}
