\noindent\textbf{Proposition:}\par
\noindent Assume $g\in\mathcal{L}^2$ and adapted to a filtration, then:\par
\begin{enumerate}[leftmargin=*]
  \item $\E\left(\int_{0}^{t}g_sdW_s\right) = 0$
  \item $\E\left(\left(\int_{0}^{t}g_sdW_s\right)^2\right) = 0 = \int_{0}^{t}\E(g_s^2)dW_s$ (Ito isometry)
  \item $X_t = \int_{0}^{t}g_sdW_s$, then $X_t$ is $\mathcal{F}^W$-adapted
\end{enumerate}
\par\bigskip
\begin{prf}[]{}
  Assume $g$ is simple (if it was not, then approximate using step functions).
  \par\bigskip
  \begin{enumerate}[leftmargin=*]
    \item
      \begin{equation*}
        \begin{gathered}
          \E\left(\int_{0}^{t}g_sdW_s\right) = 0 = \E\left(\sum_{k=1}^{n-1}g_{t_k}(W_{t_{k+1}}-W_{t_k})\right) = \sum_{k=0}^{n-1}\E\left(\underbrace{g_{t_k}}_{\text{indep.}}\underbrace{(W_{t_{k+1}}-W_{t_k})}_{\text{indep.}}\right)\\
          = \sum_{k=0}^{n-1}\E(g_{t_k})\E\underbrace{\left(W_{t_{k+1}}-W_{t_k}\right)}_{\sim N(0,\sigma^2)} = 0
        \end{gathered}
      \end{equation*}
      \par\bigskip
    \item This is the variance of a stochastic integral:
      \begin{equation*}
        \begin{gathered}
          \E\left(\left(\sum_{k=0}^{n-1}g_{t_k}(W_{t_{k+1}}-W_{t_k})\right)^2\right) = \E\left(\sum_{k=0}^{n-1}g_{t_k}^2(W_{t_{k+1}}-W_{t_j})\right)^2 + 2\sum_{j<k}\underbrace{g_{t_k}g_{t_j}}_{\in\mathcal{F}_{t_k}}\underbrace{(W_{t_{k+1}}-W_{t_k})}_{\text{indep. of } \mathcal{F}_{t_k}}\underbrace{(W_{t_{j+1}}W_{t_j})}_{\in\mathcal{F}_{t_k}}\\
          = \sum_{k=0}^{n-1}\E\left(g_{t_k}^2(W_{t_{k+1}}-W_{t_k})^2\right)+2\sum_{j<k}\E\left(g_{t_k}g_{t_j}(W_{t_{k+1}}-W_{t_k})(W_{t_{j+1}}-W_{t_j})\right)\\
          = \sum_{k=0}^{n-1}\E(g_{t_k}^2)\E\left(\underbrace{(W_{t_{k+1}}-W_{t_k})^2}_{t_{k+1}-t_k}\right) + 2\sum_{j<k}\E(\cdots)\underbrace{\E(W_{t_k+1}-W_{t_k})}_{=0}\\
          = \int_{0}^{t}\E(g_{t_k}^2)dW_s
        \end{gathered}
      \end{equation*}
  \end{enumerate}
\end{prf}
\par\bigskip
\subsection{Properties of the stochastic integarl}\hfill\\
\noindent\textbf{Examples:}\par
\noindent $\int_{0}^{t}1dW_s = W_t-W_0=W_t$, but that is $\int_{0}^{t}W_sdW_s$? $W_s$ is not piecewise constant, but we may approximate it by letting $g_t^n = W_{t_k}$ for $t\in[t_k,t_{k+1})$. What happens here is essentially discretisation but for finer and finer time.\par
\noindent This yields the approximation
\begin{equation*}
  \begin{gathered}
    \int_{0}^{t}\E\left((g_s^n-W_s)^2\right)ds = \sum_{k=0}^{n-1}\int_{t_k}^{t_{k+1}}\underbrace{\E\left((W_s-W_{t_k})^2\right)}_{s-t_k}\leftarrow\quad\text{variance of increment of BM}\\
    = \sum_{k=0}^{n-1}\int_{t_k}^{t_{k+1}}(s-t_k)ds = \sum_{k=0}^{n-1}\dfrac{1}{2}(t_{k+1}-t_k)^2 = \sum_{k=0}^{n-1}\dfrac{1}{2}\Delta t\\
    \Delta t = \dfrac{t}{n}\Rightarrow \dfrac{1}{2}(\Delta t)^2\dfrac{t}{\Delta t} = \dfrac{\Delta t}{2}t \to0\quad\text{as } n\to\infty\\
    \Rightarrow \sum_{k=0}^{n-1}W_{t_k}(W_{t_{k+1}}-W_{t_k}) = \dfrac{1}{2}\sum_{k=0}^{n-1}\left(W_{t_{k+1}}^2-W_{t_k}^2(W_{t_{k+1}}-W_{t_k})^2\right) = \dfrac{1}{2}W_{t_n}-\underbrace{\dfrac{1}{2}\sum_{k=0}^{n-1}(W_{t_{k+1}}-W_{t_k})^2}_{I_n}
  \end{gathered}
\end{equation*}
\par\bigskip
\noindent We claim $I_n\to t$ as $n\to\infty$:
\begin{equation*}
  \begin{gathered}
    \E(I_n) = \underbrace{\E\left(\sum_{k=0}^{n-1}(W_{t_{k+1}}-W_{t_k})^2\right)}_{\text{2nd moment}} = \sum_{k=0}^{n-1}(t_{k+1}-t_k) = t_n = t
  \end{gathered}
\end{equation*}\par
\noindent Need to check $\E((I_n-t)^2) = 0$:
\begin{equation*}
  \begin{gathered}
    \E\left((\sum_{k=0}^{n-1}(W_{t_{k+1}}-W_{t_k})^2-\overbrace{(t_{k+1}-t_k)}^{\Delta t})\right)^2 \\
    = \sum_{k=0}^{n-1}\E\left(\left((W_{t_{k+1}}-W_{t_k})^2-\Delta t\right)^2\right) +\sum_{j\neq k}\E\left(((W_{t_{k+1}}-W_{t_k})^2-\Delta t)((W_{t_{j+1}}-W_{t_j})-\Delta t)\right)\\
    = \sum_{j\neq k}\E\left((W_{t_{k+1}}W_{t_k})^4\right)-(\Delta t)^2 = \sum_{k=0}^{n-1}2(\Delta t)^2\sim\Delta t \to0
  \end{gathered}
\end{equation*}\par
\noindent hus, $I_n\to t$ as $n\to\infty$, so
\begin{equation*}
  \begin{gathered}
    \int_{0}^{t}W_sdW_s = \dfrac{1}{2}W_t^2-\dfrac{t}{2}
  \end{gathered}
\end{equation*}
\par\bigskip
\noindent\textbf{Remark:}\par
\noindent Lets prove if $X\sim N(0,\sigma)$, then $\E(X^4) = 3\sigma^2$
\begin{equation*}
  \begin{gathered}
    \E(X^4) = \int z^4\dfrac{1}{\sqrt{2\pi}\sigma}\text{exp}\left\{\dfrac{-z^2}{2\sigma^2}\right\}\stackrel{\text{parts}}{\Rightarrow} -\left[z^3\dfrac{1}{\sqrt{2\pi}\sigma}\text{exp}\left\{-z^2/2\sigma^2\right\}\right]_{-\infty}^\infty-\int 3z^2\dfrac{\sigma^2}{\sqrt{2\pi}\sigma}\text{exp}\left\{-z^2/2\pi\sigma^3\right\}dz\\
    = 3\sigma^2\cdot\underbrace{\int z^2\dfrac{1}{\sqrt{2\pi}\sigma}\text{exp}\left\{-z^2/2\sigma^2\right\}}_{\sigma^2} = 3\sigma^4
  \end{gathered}
\end{equation*}
\par\bigskip
\section{Martingales}
Let $\mathcal{F}_t$ be a filtration, "information generated by B; up to a time $t$".\par
\noindent If $Y$ is a random variable, then $\E(Y\mid \mathcal{F}_t)$ is the conditional expectation given all information up to time $t$
\par\bigskip
\noindent\textbf{Example:}
\begin{equation*}
  \begin{gathered}
    \E(W_s\mid\mathcal{F}_t) = W_t
  \end{gathered}
\end{equation*}
\par\bigskip
\begin{defo}[Martingale]{} 
  A process $X$ is a martingale if $X$ is $\mathcal{F}_t$-adapted. $X_t$ integrable, i.e\par
  \begin{itemize}
    \item $\E(\left|X_t\right|)<\infty\quad\forall t$
    \item $\E(X_s\mid\mathcal{F}_t) = X_t$ for $s>t$
  \end{itemize}
\end{defo}
\par\bigskip
\noindent\textbf{Example:}\par
\noindent $W_t$ is a martingale, $W_t^2-t$ is a martingale since
\begin{equation*}
  \begin{gathered}
    Y_t := W_t^2-t\qquad \E(Y_t\mid\mathcal{F}_s) = \E(W_t^2-t\mid\mathcal{F}_s)\\
    = \E((W_t-W_s)^2+2W_sW_t-W_s^2\mid\mathcal{F}_s)-t\\
    = t-s+2\E(W_sW_t\mid\mathcal{F}_s)-\E(W_s^2\mid\mathcal{F}_s)-t = 2W_s\underbrace{\E(W_t\mid\mathcal{F}_s)}_{W_s}W_s^2-s\\
    = W_s^2-s = Y_s
  \end{gathered}
\end{equation*}
\noindent $Y_t = \int_{0}^{t}g_udW_u$ is a martingale since:
\begin{equation*}
  \begin{gathered}
    \E(Y_t\mid\mathcal{F}_s) = \E\left(\int_{0}^{s}g_udW_u\mid\mathcal{F}_s\right)+\E\left(\int_{s}^{t}g_udW_u\mid\mathcal{F}_s\right) = \int_{0}^{s}g_udW_u = Y_s
  \end{gathered}
\end{equation*}\par
\noindent However, $W_t^3$ is \textit{not} a martingale:
\begin{equation*}
  \begin{gathered}
    \E(W_t^3\mid\mathcal{F}_s) = \E(W_s^3+(W_t-W_s)^3-3W_tW_s^2+3W_t^2W_s\mid\mathcal{F}_s)\\
    = W_s^3+0-3W_s^2\underbrace{\E(W_t\mid\mathcal{F}_s)}_{W_s} + 3W_s\underbrace{\E(W_t^2\mid\mathcal{F}_s)}_{t-s+W_s^2}\\
    = W_s^3+3(t-s)W_s\neq W_s^3
  \end{gathered}
\end{equation*}
\par\bigskip
\noindent\textbf{Remark:} A martingale is a "fair game"
\par\bigskip
\subsection{Itos formula}\hfill\\
\noindent Assume 
\begin{equation*}
  \begin{gathered}
    X_t = a+\int_{0}^{t}\mu_sds + \int_{0}^{t}\sigma_sdW_s
  \end{gathered}
\end{equation*}\par
\noindent for some adapted process $\mu_t$ and $\sigma_t$. Short-hand notation $\begin{cases}dX_t = \mu_tdt+\sigma_tdW_t\\X_0=a\end{cases}$
\par\bigskip
\noindent Let $f(t,x)$ be a $C^{1,2}$-function and define $Z_t = f(t,X_t)$, what does $dZ_t$ look like?
\par\bigskip
\noindent\textbf{Recall:}
\begin{equation*}
  \begin{gathered}
    \int_{0}^{t}W_sdW_s = \dfrac{W_t^2}{2}-\dfrac{t}{2}
  \end{gathered}
\end{equation*}\par
\noindent so $W_t^2 = t+2\int_{0}^{t}W_sdW_s$, thus 
\begin{equation*}
  \begin{gathered}
    d(W_t^2) = dt +2W_tdW_t
  \end{gathered}
\end{equation*}\par
\noindent Fix $n$ and let $t_k = \dfrac{k}{n}t$\par
\noindent Let $\Delta W_{t_k} = W_{t_{k+1}}-W_{t_k}$ and consider
\begin{equation*}
  \begin{gathered}
    S_n = \sum_{k=0}^{n-1} \left(\Delta W_{t_k}\right)^2
  \end{gathered}
\end{equation*}\par
\noindent We have 
\begin{equation*}
  \begin{gathered}
    \E(S_n) = \sum_{k=0}^{n-1}\E\left(\left(\Delta W_{t_k}\right)^2\right) = \sum_{k=0}^{n-1}\dfrac{t}{n} = t
  \end{gathered}
\end{equation*}\par
\noindent and
\begin{equation*}
  \begin{gathered}
    \text{Var}\left(S_n\right) \stackrel{\text{indep.}}{=} \sum_{k=0}^{n-1}\text{Var}\left(\left(\Delta W_{t_k}\right)^2\right) = n\text{Var}\left(\left(\Delta W_{t_0}\right)^2\right) = n\cdot2\dfrac{t^2}{n^2}\to0\quad\text{ as } n\to\infty
  \end{gathered}
\end{equation*}\par
\noindent Thus $S_n\to t$ as $n\to\infty$ (in $\mathcal{L}^2$). This motivates to write
\begin{equation*}
  \begin{gathered}
    \int_{0}^{t}(dW_s^2) = t\\
    \Lrarr dW_t^2 = dt
  \end{gathered}
\end{equation*}
